new/proof/time.v
@@ -57,10 +57,17 @@ Axiom wp_Time__Add : ∀ (t : time.Time.t) (d : time.Duration.t),
     t @ time.Time.id @ "Add" #d
   {{{ (t : time.Time.t), RET #t; True }}}.
 
-Axiom wp_arbitraryTime :
+Lemma wp_arbitraryTime :
   {{{ True }}}
     time.arbitraryTime #()
   {{{ (t: time.Time.t), RET #t; True }}}.
+Proof.
+  wp_start.
+  wp_call.
+  change time.time.__Time with time.Time.
+  wp_apply wp_ArbitraryInt as "%x".
+  by iApply "HΦ".
+Qed.
 
 Lemma wp_After (d : time.Duration.t) :
   {{{ is_pkg_init time }}}
